If you've got enough RAM, type checking of addition is also provably decidable.

ott/coq/AilTyping.v
@@ -1111,6 +1111,33 @@ Proof.
         | inversion 1; isAssignable_neg_tac].
 Qed.
 
+Definition isPointerToCompleteObject_fun ty : bool :=
+  match ty with
+  | Pointer _ t => isComplete_fun t
+  | _           => false
+  end.
+
+Lemma isPointerToCompleteObject_correct t :
+  boolSpec (isPointerToCompleteObject_fun t)
+           (isPointer t * {qs : qualifiers & {ty : type & (t = Pointer qs ty) * isComplete ty}}).
+Proof.
+  do 2 unfold_goal;
+  repeat match goal with
+  | [|- isComplete_fun ?t = _ -> _] => case_fun (isComplete_fun_correct t)
+  | [|- neg _] => intros [? [? [? [? ?]]]]
+  | [H : isPointer ?t |- False] =>
+      match t with
+      | Pointer _ _ => fail 1
+      | _ => now inversion H
+      end
+  | [Heq : Pointer _ _ = Pointer _ _ |- False] => inversion Heq; intros; subst; contradiction
+  | [|- _ * _] => split
+  | [|- isPointer (Pointer _ _)] => constructor
+  | [|- {_ : _ & _}] => eexists; eexists; split; [reflexivity | assumption]
+  | _ => context_destruct
+  end.
+Qed.
+
 Fixpoint eType_find (P:impl) (G:gamma) (S:sigma) e {struct e} : option typeCategory :=
   match e with
   | Var id =>
@@ -1189,10 +1216,42 @@ Fixpoint eType_find (P:impl) (G:gamma) (S:sigma) e {struct e} : option typeCateg
             else None
       | _, _ => None
       end
-  | Binary e1 (Arithmetic Mul) e2 =>
+  | Binary e1 (Arithmetic (Mul  as aop)) e2
+  | Binary e1 (Arithmetic (Div  as aop)) e2
+  | Binary e1 (Arithmetic (Mod  as aop)) e2
+  | Binary e1 (Arithmetic (Band as aop)) e2
+  | Binary e1 (Arithmetic (Xor  as aop)) e2
+  | Binary e1 (Arithmetic (Bor  as aop)) e2 =>
       match eType_find P G S e1 >>= expressionType_find, eType_find P G S e2 >>= expressionType_find with
-      | Some ty1, Some ty2 => if isBinaryArithmetic_fun ty1 Mul ty2
+      | Some ty1, Some ty2 => if isBinaryArithmetic_fun ty1 aop ty2
                                 then option_map ExpressionType (isUsualArithmetic_find P ty1 ty2)
+                                else None
+      | _       , _        => None
+      end
+  | Binary e1 (Arithmetic (Shl  as aop)) e2
+  | Binary e1 (Arithmetic (Shr  as aop)) e2 =>
+      match eType_find P G S e1 >>= expressionType_find, eType_find P G S e2 >>= expressionType_find with
+      | Some ty1, Some ty2 => if isBinaryArithmetic_fun ty1 aop ty2
+                                then option_map ExpressionType (isPromotion_find P ty1)
+                                else None
+      | _       , _        => None
+      end
+  | Binary e1 (Arithmetic (Add  as aop)) e2 =>
+      match eType_find P G S e1 >>= expressionType_find, eType_find P G S e2 >>= expressionType_find with
+      | Some (Pointer qs1 ty1), Some ty2
+      | Some ty2              , Some (Pointer qs1 ty1) => if andb (isComplete_fun ty1) (isInteger_fun ty2)
+                                                            then Some (ExpressionType (Pointer qs1 ty1))
+                                                            else None
+      | Some ty1              , Some ty2               => if isBinaryArithmetic_fun ty1 aop ty2
+                                                            then option_map ExpressionType (isUsualArithmetic_find P ty1 ty2)
+                                                            else None
+      | _                     , _                      => None
+      end
+  | Binary e1 And e2
+  | Binary e1 Or  e2 =>
+      match eType_find P G S e1 >>= expressionType_find, eType_find P G S e2 >>= expressionType_find with
+      | Some ty1, Some ty2 => if andb (isScalar_fun ty1) (isScalar_fun ty2)
+                                then Some (ExpressionType (Basic (Integer (Signed Int))))
                                 else None
       | _       , _        => None
       end
@@ -1226,7 +1285,29 @@ Proof.
   intros Hdisjoint.
   destruct e; unfold eType_find; fold eType_find.
   Focus 2.
+
   repeat match goal with
+  | [H : boolSpec true  _ |- _] => rewrite boolSpec_true  in H
+  | [H : boolSpec false _ |- _] => rewrite boolSpec_false in H
+  | [H : isBinaryArithmetic Void Add _ |- _] => inversion_clear H
+  | [H : isBinaryArithmetic _ Add Void |- _] => inversion_clear H
+  | [H : isBinaryArithmetic (Array _ _) Add _ |- _] => inversion_clear H
+  | [H : isBinaryArithmetic _ Add (Array _ _) |- _] => inversion_clear H
+  | [H : isBinaryArithmetic (Pointer _ _) Add _ |- _] => inversion_clear H
+  | [H : isBinaryArithmetic _ Add (Function _ _) |- _] => inversion_clear H
+  | [H : isBinaryArithmetic (Function _ _) Add _ |- _] => inversion_clear H
+  | [H : isBinaryArithmetic _ Add (Pointer _ _) |- _] => inversion_clear H
+  | [H : isComplete Void |- _ ] => inversion H
+  | [H : isObject (Function _ _) |- _ ] => inversion H
+  | [H : isInteger    Void           |- _ ] => inversion H
+  | [H : isInteger    (Array _ _) |- _ ] => inversion H
+  | [H : isInteger    (Function _ _) |- _ ] => inversion H
+  | [H : isInteger    (Pointer  _ _) |- _ ] => inversion H
+  | [H : isArithmetic Void           |- _ ] => inversion_clear H
+  | [H : isArithmetic (Array _ _) |- _ ] => inversion_clear H
+  | [H : isArithmetic (Function _ _) |- _ ] => inversion_clear H
+  | [H : isArithmetic (Pointer  _ _) |- _ ] => inversion_clear H
+  | [H : isAssignable P G S (pointerConvert _) _ |- False] => inversion_clear H
   | [|- lookup_id ?E ?id = ?o -> _] =>
       case_fun (lookup_id_correct E id)
   | [|- eType_find P G S ?e = ?o -> _] =>
@@ -1293,6 +1374,7 @@ Proof.
   | [|- isArithmetic_fun ?t           = ?o -> _] => is_var o; case_fun (isArithmetic_fun_correct t)
   | [|- isComplete_fun ?t           = ?o -> _] => is_var o; case_fun (isComplete_fun_correct t)
   | [|- isObject_fun ?t           = ?o -> _] => is_var o; case_fun (isObject_fun_correct t)
+  | [|- isScalar_fun ?t           = ?o -> _] => is_var o; case_fun (isScalar_fun_correct t)
   | [|- isInteger_fun ?t           = ?o -> _] => is_var o; case_fun (isInteger_fun_correct t)
   | [|- isReal_fun ?t           = ?o -> _] => is_var o; case_fun (isReal_fun_correct t)
   | [|- isPointer_fun ?t           = ?o -> _] => is_var o; case_fun (isPointer_fun_correct t)
@@ -1328,19 +1410,22 @@ Proof.
       let Heq := fresh in
       assert (t1 = t2) as Heq by (eapply expressionType_unique_lvalue_inj; eauto);
       try (congruence || (try injection Heq; intros); subst)
-  | [ Hunique : forall _, eType P G S ?e _ -> ExpressionType ?t1 = _
-    , H1 : expressionType P G S ?e (pointerConvert ?t1)
+  | [ Hunique : forall _, eType P G S ?e _ -> ExpressionType ?t = _
+    , _   : expressionType_find (ExpressionType ?t) = Some ?t1
+    , H1 : expressionType P G S ?e ?t1
     , H2 : expressionType P G S ?e ?t2         |- _ ] =>
-      is_var t2;
+      notSame t1 t2;
       let Heq := fresh in
-      assert (pointerConvert t1 = t2) as Heq by (eapply (expressionType_unique_expression_inj (eType_unique_instance Hunique)); eauto);
+      assert (t1 = t2) as Heq by (eapply (expressionType_unique_expression_inj (eType_unique_instance Hunique)); eauto);
       try (congruence || (try injection Heq; intros); subst)
+(*
   | [ _  : expressionType P G S ?e ?t1
     , _  : expressionType P G S ?e ?t2         |- _ ] =>
       notSame t1 t2;
       let Heq := fresh in
       assert (t1 = t2) as Heq by (eapply expressionType_unique_expression_inj; eauto);
       try (congruence || (try injection Heq; intros); subst)
+*)
   | [H : isPromotion P ?t1 ?t2 |- _ ] => notHyp (isPromotion_find P t1 = Some t2); set (isPromotion_find_unique P t1 t2 H); try congruence
   | [H : lvalueConversion ?t1 ?t2 |- _ ] => notHyp (lvalueConversion_find t1 = Some t2); set (lvalueConversion_find_unique t1 t2 H); try congruence
   | [H : isUsualArithmetic P ?t1 ?t2 ?t3 |- _ ] => notHyp (isUsualArithmetic_find P t1 t2 = Some t3); set (isUsualArithmetic_find_unique H); try congruence
@@ -1351,9 +1436,13 @@ Proof.
   | [ Hunique : forall _, eType P G S ?e _ -> ExpressionType _ = _, H : eType P G S ?e (ExpressionType ?t) |- _] =>
       discriminate (Hunique _ H) || (einjection (Hunique _ H); congruence)
   | [|- forall _, eType P G S (Binary _ Comma _) _ -> _ = _] => inversion_clear 1; now auto
-  | [|- forall _, eType P G S (Binary _ (Arithmetic Mul) _) _ -> _ = _] => inversion 1; subst
+  | [|- forall _, eType P G S (Binary _ (Arithmetic _) _) _ -> _ = _] => inversion 1; subst
+  | [|- forall _, eType P G S (Binary _ And _) _ -> _ = _] => inversion 1; subst
+  | [|- forall _, eType P G S (Binary _ Or _) _ -> _ = _] => inversion 1; subst
   | [|- forall _, neg (eType P G S (Binary _ Comma _) _)] => inversion 1; subst
-  | [|- forall _, neg (eType P G S (Binary _ (Arithmetic Mul) _) _)] => inversion 1; subst
+  | [|- forall _, neg (eType P G S (Binary _ (Arithmetic _) _) _)] => inversion 1; subst
+  | [|- forall _, neg (eType P G S (Binary _ And _) _)] => inversion 1; subst
+  | [|- forall _, neg (eType P G S (Binary _ Or _) _)] => inversion 1; subst
   | [|- forall _, neg (eType P G S (Unary _ _) _)] => inversion 1; subst
   | [|- forall _, neg (eType P G S (Call _ _) _)] => inversion 1; subst
   | [|- forall _, neg (eType P G S (Assign _ _) _)] => inversion 1; subst
@@ -1366,8 +1455,7 @@ Proof.
   | [|- forall _, eType P G S (Var _) _ -> _ = _] => inversion_clear 1
   | [|- forall _, eType P G S (Call _ _) _ -> _ = _] => inversion_clear 1
   | [|- forall _, eType P G S (Assign _ _) _ -> _ = _] => inversion_clear 1
-  | [|- eType _ _ _ (Var _) (LvalueType _ _) ] =>
-      now my_auto
+  | [|- eType _ _ _ (Var _) (LvalueType _ _) ] => now my_auto
   | [ L1 : Lookup ?G ?id _
     , L2 : Lookup ?S ?id _ |- _ ] =>
       destruct (Hdisjoint id _ _ L1 L2)
@@ -1378,31 +1466,32 @@ Proof.
     ,_ : forall _, neg (Lookup ?S ?id _) |- forall _, neg (eType _ ?G ?S (Var ?id) _)] =>
       inversion 1; now firstorder
   | [ _ : forall _, neg (eType P G S ?e _) , H : expressionType P G S ?e _ |- _] => inversion H
-  | [H : isComplete Void |- _ ] => inversion H
-  | [H : isObject (Function _ _) |- _ ] => inversion H
-  | [H : isAssignable P G S (pointerConvert _) _ |- False] => inversion_clear H
-  | _ => boolSpec_simpl
   end.
-  Focus 4.
+
+
+
+
+
+  | [ Hunique : forall _, eType P G S ?e _ -> ExpressionType ?t1 = _
+    , H1 : expressionType P G S ?e ?t1
+    , H2 : expressionType P G S ?e ?t2         |- _ ] =>
+      notSame t1 t2;
+      let Heq := fresh in
+      assert (t1 = t2) as Heq by (eapply (expressionType_unique_expression_inj (eType_unique_instance Hunique)); eauto);
+      try (congruence || (try injection Heq; intros); subst)
+
 
   match goal with
+  | [ Hunique : forall _, eType P G S ?e _ -> ExpressionType ?t = _
+    , _   : expressionType_find (ExpressionType ?t) = Some ?t1
+    , H1 : expressionType P G S ?e ?t1
+    , H2 : expressionType P G S ?e ?t2         |- _ ] =>
+      is_var t2;
+      let Heq := fresh in
+      assert (t1 = t2) as Heq by (eapply (expressionType_unique_expression_inj (eType_unique_instance Hunique)); eauto);
+      try (congruence || (try injection Heq; intros); subst)
   end.
 
-
-
-      
-
-
-  match goal with
-
-  end.
-
-      assert (t1 = t2) as Heq by (eapply expressionType_unique_expression_inj; eauto);
-  match goal with
-  | _ => 
-  | _ => idtac
-  end.
-  
 Qed.
 
 (* defns JsType *)
